dafny/session-13/adts-1.dfy
@@ -123,7 +123,7 @@ function inorder<T> (t: Tree<T>): seq<T>
 function rev <T> (s:seq<T>): (res:seq<T>)
 {
    if s==[] then []
-            else rev(s[1..]) + [s[0]]
+   else rev(s[1..]) + [s[0]]
 }
 
 
@@ -162,219 +162,87 @@ function mset(t:Skew): multiset<int>
 
 // 1. Prove the following lemma:
 
+lemma sortedHeadLE (l:List<int>)
+requires l != Nil
+requires sorted(l)
+ensures forall e | e in elems(l) :: l.head <= e
+{}
+
 lemma sortedConcat (l1:List<int>, l2:List<int>)
 requires sorted(l1) && sorted(l2) 
 requires forall x,y | x in elems(l1) && y in elems(l2) :: x <= y
 ensures sorted(concat(l1,l2))
+{
+   match l1
+      case Nil          => {}
+      case Cons(head1,tail1)   =>
+         match l2
+            case Nil          => {}
+            case Cons(head2,tail2)   =>
+               {
+                  assert l2.head in elems(l2);
+                  assert forall e | e in elems(l1) :: e <= head2;
+                  sortedHeadLE(l2);
+                  assert forall e | e in elems(l2) :: head2 <= e;
+                  assert forall e | e in elems(tail1) :: e in elems(l1);
+               }
+}
 
 // 2. Prove the following lemma:
 
-// lemma reverseConcat<T>(head:T, tail:List<T>)
-// ensures reverse(concat(tail, Cons(head, Nil))) == Cons(head, reverse(tail))
-// {}
+// reverse(l) == concat(reverse(xs),Cons(x,Nil))
 
-// lemma reverseIdemp<T> (l:List<T>)
-// ensures reverse(reverse(l)) == l {
-//     if l.Cons? {
-//         calc == {
-//             reverse(reverse(l));
-//             reverse(concat(reverse(l.tail), Cons(l.head, Nil)));
-//             { reverseConcat(l.head, reverse(l.tail)); }
-//             Cons(l.head, reverse(reverse(l.tail)));
-//             { reverseIdemp(l.tail); }
-//             Cons(l.head, l.tail);
-//             l;
-//         }
-//     }
-// }
+lemma reverseHeadConcat<T> (head:T, tail:List<T>)
+ensures reverse(concat(tail, Cons(head, Nil))) == Cons(head, reverse(tail))
+{}
+
+lemma reverseIdemp<T> (l:List<T>)
+ensures reverse(reverse(l)) == l
+{
+   match l
+      case Nil             => {}
+      case Cons(head,tail) =>
+         {
+            calc == {
+               reverse(reverse(l));
+               reverse(concat(reverse(tail), Cons(head,Nil)));
+               ==
+               {reverseHeadConcat(head, reverse(tail)); }
+               l;
+            }
+         }
+}
 
 
 // 3. Prove the following lemma:  # LEMMA TO BE PROVED :: 3  <------
 
-function last<T> (l:List<T>): List<T>
-requires l != Nil
-ensures drop(length(l)-1,l) == last(l)
-ensures last(l).tail == Nil
-{
-   match l
-      case Cons(x,Nil) => l
-      case Cons(x,xs)  => last(xs)
-}
+// reverse(l) == concat(reverse(xs),Cons(x,Nil))
 
-lemma concatReverseLast<T> (l1:List<T>, l2:List<T>)
-requires l1 != Nil && l2 != Nil
-ensures last(concat(l1,l2)) == last(l2)
+lemma dropReverse<T> (l1:List<T>, l2:List<T>, n:nat)
+requires length(l1) >= n
+ensures concat(drop(n, l1), l2) == drop(n, concat(l1,l2))
 {}
-
-lemma lastTail<T> (l:List<T>)
-requires l != Nil
-ensures l.head == last(reverse(l)).head
-{
-   match l
-      case Cons(x,Nil) => 
-         assert l.head == last(reverse(l)).head;
-      case Cons(x,xs)  =>
-         lastTail(xs);
-         var l1 := concat(reverse(xs),Cons(x,Nil));
-         assert reverse(l) == l1;
-         concatReverseLast(reverse(xs),Cons(x,Nil));
-         assert last(l1) == last(Cons(x,Nil));
-}
-
-lemma lastConcat<T> (l1: List<T>, x:T)
-requires l1 != Nil
-ensures last(concat(l1,Cons(x,Nil))) == Cons(x,Nil)
-{}
-
-lemma dropKeepLast<T> (l:List<T>)
-requires l != Nil
-ensures drop(length(l)-1,l) == Cons(last(l).head,Nil)
-{}
-
-lemma lastDrop<T> (n:nat, l:List<T>)
-requires l != Nil
-requires length(l) > n >= 1
-ensures last(drop(length(l)-n,l)) == last(l)
-{
-   match l
-      case Cons(x,Nil) =>
-         assert last(drop(length(l)-n,l)) == last(l);
-      case Cons(x,xs)  =>
-         if (n==1) {
-            dropKeepLast(l);
-         } else {
-            assert drop(length(l)-n,Cons(x,xs)) == drop(length(xs)-n,xs);
-         }
-}
-
-lemma dropConcatLength<T> (l1:List<T>,l2:List<T>)
-requires l1 != Nil && l2 != Nil
-ensures drop(length(l1),concat(l1,l2)) == l2
-{}
-
-lemma lastReverse<T> (l:List<T>)
-requires l != Nil
-ensures reverse(l) == concat(reverse(l.tail), Cons(l.head,Nil))
-{}
-
-lemma dropReverse1<T> (l:List<T>)
-requires l != Nil
-ensures drop(1,reverse(l)) == reverse(take(length(l)-1,l))
-{
-   match l
-      case Cons(x,Nil) =>
-         assert drop(1,reverse(l)) == reverse(take(length(l)-1,l));
-      case Cons(x,xs)  =>
-         dropReverse1(xs);
-}
-
-lemma dropReverse11<T> (l:List<T>)
-requires l != Nil
-requires length(l) >= 2
-ensures drop(1,reverse(l)) == concat(drop(1,reverse(l.tail)),Cons(l.head,Nil))
-{
-   match l
-      case Cons(x,xs)  =>
-         if (length(xs) == 1) {
-            assert drop(1,xs) == Nil;
-         }
-}
-
-
-lemma dropReverse2<T> (l:List<T>)
-requires l != Nil
-ensures drop(length(l)-1,reverse(l)) == Cons(l.head,Nil)
-{
-   match l
-      case Cons(x,Nil) =>
-         assert drop(length(l)-1,reverse(l)) == Cons(l.head,Nil);
-      case Cons(x,xs)  =>
-         dropReverse2(xs);
-         dropConcatLength(reverse(xs),Cons(x,Nil));
-}
-
-lemma concatReverse<T> (x:T, l:List<T>)
-requires l != Nil
-ensures reverse(Cons(x,l)) == concat(reverse(l),Cons(x,Nil))
-ensures last(concat(reverse(l),Cons(x,Nil))) == Cons(x,Nil)
-{
-   lastConcat(reverse(l),x);
-   assert last(concat(reverse(l),Cons(x,Nil))) == Cons(x,Nil);
-}
-
-lemma dropStep<T> (n:nat, l:List<T>)
-requires l != Nil
-requires length(l) > n && n >= 1
-ensures drop(length(l)-n,l) == drop(length(l.tail)-n,l.tail)
-{}
-
-lemma dropConcatReverse<T> (n:nat, l:List<T>)
-requires l != Nil
-requires length(l) > n && n >= 1
-ensures drop(length(l)-n,reverse(l)) ==
-         concat(drop(length(l)-n,reverse(l.tail)),Cons(l.head,Nil));
-{
-   match l
-      case Cons(x,Nil) =>
-         assert drop(length(l)-n,reverse(l)) ==
-                concat(drop(length(l.tail)-n+1,reverse(l.tail)),Cons(l.head,Nil));
-      case Cons(x,xs)  =>
-         if (n==1) {
-            concatReverse(x,xs);
-         }
-         else {
-            dropConcatReverse(n-1,xs);
-            assert drop(length(l)-n,reverse(xs)) == concat(drop(length(l)-n,reverse(xs.tail)),Cons(xs.head,Nil));
-            
-            // concatReverse(x,xs);
-            // assert last(reverse(Cons(x,xs))) == Cons(x,Nil);
-            // assert last(drop(length(xs)-n+1,reverse(Cons(x,xs)))) == Cons(x,Nil);
-            
-            assert drop(length(l)-n,reverse(l)) == drop(length(xs)-n+1,reverse(Cons(x,xs)));
-            assert length(xs) - n + 1 < length(l);
-
-            dropStep(n,reverse(l));
-            // assert drop(length(xs)-n+1,reverse(Cons(x,xs))) == concat(drop(length(xs)-n+1,reverse(xs)),Cons(x,Nil));
-            
-         }
-}
 
 lemma takeReverse<T> (n: nat, l:List <T>)
 requires length(l) >= n
 ensures reverse(take(n,l)) == drop(length(l)-n,reverse(l))
 {
    match l
-      case Nil =>
-         assert reverse(take(n,l)) == drop(length(l)-n,reverse(l));  // Both sides are Nil
-      case Cons(x,Nil) =>
-         assert reverse(take(n,l)) == drop(length(l)-n,reverse(l));  // Both sides are Cons(x,Nil)
-      case Cons(x,xs) =>
-         if (n==0) {
-            assert reverse(take(n,l)) == drop(length(l)-n,reverse(l));
-         }
-         else if (n==1) {
-            lastTail(l);
-         } else if (length(l) == n) {
-            assert reverse(take(n,l)) == drop(length(l)-n,reverse(l)) == reverse(l);
-         } else {
-            assert length(l) > n >= 2;
-            takeReverse(n-1,xs);
-            assert reverse(take(n-1,xs)) == drop(length(l)-n,reverse(xs));  // Inductive step
-
-            // assert take(n,l) == Cons(x,take(n-1,xs));
-            // assert reverse(take(n,l)) == reverse(Cons(x,take(n-1,xs)));
-            concatReverse(x,take(n-1,xs));
-            // assert last(reverse(Cons(x,take(n-1,xs)))) == Cons(x,Nil);
-            assert reverse(Cons(x,take(n-1,xs))) == concat(reverse(take(n-1,xs)),Cons(x,Nil));  // Key point
-
-            assert reverse(take(n,l)) == concat(drop(length(l)-n,reverse(xs)),Cons(x,Nil));
-
-            assert drop(length(l)-n,reverse(l)) == drop(length(l)-n,reverse(Cons(x,xs)));
-            assert length(l) == length(xs)+1;
-
-            // dropConcatReverse(n,l);
-            // assert concat(drop(length(l)-n,reverse(xs)),Cons(x,Nil)) == drop(length(l)-n,reverse(Cons(x,xs)));
-            // assert reverse(take(n,l)) == drop(length(l)-n,reverse(l));
+      case Nil                => {}
+      case Cons(head, tail)   =>
+         if n == 0
+            {}
+         else
+            {
+               calc == {
+                  reverse(take(n,Cons(head, tail)));
+                  reverse(Cons(head, take(n-1, tail)));
+                  concat(reverse(take(n-1, tail)), Cons(head, Nil));
+                  { takeReverse(n-1, tail); }
+                  concat(drop(length(tail)-(n-1), reverse(tail)), Cons(head, Nil));
+                  { dropReverse(reverse(tail), Cons(head, Nil), length(tail)-(n-1)); }
+                  drop(length(l)-n, reverse(l));
+            }
          }
 }
 
@@ -383,9 +251,104 @@ ensures reverse(take(n,l)) == drop(length(l)-n,reverse(l))
 
 function mirror<T>(t:Tree<T>):(res:Tree<T>)
 ensures tset(res)==tset(t)
+{
+   match t
+      case Empty        => Tree.Empty
+      case Node(l,x,r)  => Tree.Node(mirror(r), x, mirror(l))
+}
+
+lemma mirrorLemma<T> (t:Tree<T>)
+requires t != Tree.Empty
+ensures mirror(t) == Tree.Node(mirror(t.right), t.key, mirror(t.left))
+{}
+
+lemma inorderLemma<T> (t:Tree<T>)
+requires t != Tree.Empty
+ensures inorder(t) == inorder(t.left) + [t.key] + inorder(t.right)
+{}
+
+lemma revLemma<T> (s:seq<T>, x:T)
+ensures rev([x] + s) == rev(s) + [x]
+{}
+
+lemma revLemmaSeq<T> (s1:seq<T>, s2:seq<T>, x:T)
+ensures rev([x] + (s1 + s2)) == rev(s1 + s2) + [x]
+{}
+
+lemma revEmpty<T> (s:seq<T>)
+ensures [] + rev(s) == rev(s)
+{}
+
+lemma revEmpty21<T> (s:seq<T>)
+ensures s == s + []
+{}
+
+lemma revEmpty22<T> (s:seq<T>)
+ensures s == [] + s
+{}
+
+lemma revLemmaComm1<T> (s1:seq<T>, s2:seq<T>, s3:seq<T>)
+ensures s1 + (s2 + s3) == (s1 + s2) + s3
+{}
+
+lemma revLemmaComm2<T> (s1:seq<T>, s2:seq<T>, s3:seq<T>)
+ensures s1 + (s2 + s3) == s1 + s2 + s3
+{}
+
+lemma revLemma2<T> (s1:seq<T>, s2:seq<T>)
+ensures rev(s1) + rev(s2) == rev(s2 + s1)
+{
+   if |s1| == 0 {
+      revEmpty21(s2);
+      assert rev(s1) + rev(s2) == rev(s2 + s1);
+   } else {
+      if |s2| == 0 {
+         revEmpty22(s1);
+      } else {
+         calc == {
+            rev(s1) + rev(s2);
+            { assert rev(s2) == rev([s2[0]] + s2[1..]); }
+            { revLemma(s2[1..], s2[0]); }
+            rev(s1) + rev(s2[1..]) + [s2[0]];
+            { revLemma2(s1, s2[1..]); }
+            { assert rev(s1) + rev(s2[1..]) == rev(s2[1..] + s1); }
+            rev(s2[1..] + s1) + [s2[0]];
+            { revLemmaSeq(s2[1..], s1, s2[0]); }
+            rev([s2[0]] + (s2[1..] + s1));
+            { revLemmaComm2([s2[0]], s2[1..], s1); }
+            rev([s2[0]] + s2[1..] + s1);
+            { assert [s2[0]] + s2[1..] == s2; }
+            rev(s2 + s1);
+         }
+      }
+   }
+}
 
 lemma reverseMirror<T> (t: Tree<T>)
 ensures inorder(mirror(t)) == rev(inorder(t))
+{
+   match t
+      case Empty             => {}
+      case Node(l,x,r)  =>
+         {
+            calc == {
+               inorder(mirror(t));
+               { mirrorLemma(t); }
+               inorder(Tree.Node(mirror(r), x, mirror(l)));
+               { inorderLemma(Tree.Node(mirror(r), x, mirror(l))); }
+               inorder(mirror(r)) + [x] + inorder(mirror(l));
+               { reverseMirror(l); }
+               { reverseMirror(r); }
+               rev(inorder(r)) + [x] + rev(inorder(l));
+               { revLemma(inorder(r), x); }
+               rev([x] + inorder(r)) + rev(inorder(l));
+               { revLemma2(([x] + inorder(r)), inorder(l)); }
+               rev(inorder(l) + ([x] + inorder(r)));
+               { revLemmaComm2(inorder(l), [x], inorder(r)); }
+               rev(inorder(l) + [x] + inorder(r));
+            }
+         }
+}
 
 // 5. Program the function mirror of exercise 4.
 //    Program the recursive traversals preorder and postorder of a binary tree, 
@@ -415,4 +378,3 @@ ensures sortedSeq(res)
                            var right := flatten(r);
                            [x] + merge(left,right)
 }
-
