dafny/exam2021/Exercise1_fresh.dfy
@@ -1,0 +1,80 @@
+//Final Exam, June 10th, 2021
+//We want to specify and verify a method that, given an array of distinct elements, 
+//computes the number of elements that have a smaller element on their right. 
+//Example: given the array elements [2,6,8,4,9,5,10], the method must return 3
+//because elements 9, 8 and 6 have smaller elements on their right.
+
+//Your tasks are:
+
+//1.Define a predicate oneBiggerOnRight that given an array v and a valid index i
+//on that array, determines if there exists an element on i's right that is smaller 
+//than v[i]
+
+predicate oneBiggerOnRight(v: array<int>, i:int)
+reads v
+requires v.Length > 0
+requires 0 <= i < v.Length
+{
+    (exists j | i < j < v.Length :: v[j] < v[i])
+}
+
+//2.Define a function countBiggerOnRight that given an array v and a valid index i
+//on that array, returns the number of elements in segment [i..v.Length] that meet 
+//the property oneBiggerOnRight previously defined
+
+function countBiggerOnRight(v : array<int>, i:int): int
+reads v
+requires v.Length > 0
+requires 0 <= i < v.Length
+decreases v.Length - i
+{
+    if i == v.Length - 1 then
+        0
+    else
+        if oneBiggerOnRight(v, i) then
+            1 + countBiggerOnRight(v, i+1)
+        else
+            countBiggerOnRight(v, i+1)
+}
+
+//3.Using function countBiggerOnRight, specify a method
+//that receives an array v of distinct elements and returns  
+//the number of elements that have a smaller element on the right 
+
+predicate distinct(v:array<int>)
+reads v
+requires v.Length > 0
+{
+    forall i:int, j:int | 0 <= i < j < v.Length :: v[i] != v[j]
+}
+
+method mCountBiggerOnRight(v: array<int>) returns (c:int)
+requires v.Length > 0
+requires distinct(v)
+ensures c == countBiggerOnRight(v, 0)
+{
+    var i:int := v.Length - 1;
+    var m:int := v[i];
+    
+    c := 0;
+
+    while (i > 0)
+        decreases i
+        invariant 0 <= i < v.Length
+        invariant exists j | i <= j < v.Length :: m == v[j]  // It's important to demonstrate that this element (m, minimum) exists in the array
+        invariant forall k | i <= k < v.Length :: m <= v[k]  // global min
+        invariant c == countBiggerOnRight(v, i)
+    {
+        if (v[i-1] > m) {
+            c := c + 1;
+        } else {
+            m := v[i-1];
+        }
+        i := i - 1;
+    }
+}
+
+//4. Implement and verify an algorithm that solves this problem.
+//A linear time algorithm will be better valued.  
+
+
