dafny/exam2021/Exercise2_fresh.dfy
@@ -1,0 +1,143 @@
+/*
+    Final Exam, June 10th, 2021
+    Exercise on algebraic datatypes
+
+    You are given the definitions below and you are asked to represent
+    sets of integers as sorted lists of integers without duplicates
+
+    You are also given the specifications of the emptySet, singleton, union and 
+    intersection functions. Your task consists of implementing and verifying 
+    them. The cost of union and intersection should in O(n1+n2), being n1 and n2
+    the cardinals of the sets received as arguments. 
+*/
+
+datatype List<T> = Nil | Cons(head:T, tail:List<T>)
+
+predicate noDup <T> (l:List<T>)
+{
+    match l
+        case Nil        => true
+        case Cons(x,xs) => x !in elems(xs) && noDup(xs)
+}
+
+predicate sorted (l:List<int>)
+{
+    match l 
+       case Nil         => true
+       case Cons(x, xs) => 
+            match xs 
+               case Nil         => true
+               case Cons(y, ys) => x <= y && sorted(xs)
+}
+
+function elems <T> (l:List<T>) : set<T>
+{
+    match l
+       case Nil         => {}
+       case Cons(x, xs) => {x} + elems(xs)
+}
+
+///////////////////////////////////////////////////////////////
+
+function method emptySet() : (res:List<int>)
+ensures elems(res) == {}
+{
+    Nil
+}
+
+function method singleton(x:int): (res:List<int>)
+ensures elems(res) == {x} && noDup(res)
+{
+    Cons(x, emptySet())
+}
+
+function method insertSorted(l:List<int>, y:int) : (res:List<int>)
+requires sorted(l) && noDup(l)
+ensures sorted(res) && noDup(res)
+ensures elems(res) == elems(l) + {y}
+{
+    match l
+        case Nil        => singleton(y)
+        case Cons(x,xs) =>
+            if y < x then
+                lessHeadNotElems(y,l);
+                Cons(y,l)
+            else
+                if y == x then
+                    l
+                else
+                    Cons(x,insertSorted(xs,y))
+}
+
+
+function method union (l1:List<int>,l2:List<int>): (res: List<int>)
+requires sorted(l1) && sorted(l2) && noDup(l1) && noDup(l2)
+ensures sorted(res) && noDup(res)
+ensures elems(res) == elems(l1) + elems (l2)
+decreases l2
+{
+    match l1
+        case Nil            => l2
+        case Cons(x, xs)    =>
+            match l2
+                case Nil            => l1
+                case Cons(y, ys)    =>
+                    if x < y then
+                        var auxL1 := insertSorted(xs,y);
+                        assert sorted(xs);
+                        assert sorted(Cons(y,Nil));
+                        assert sorted(auxL1);
+                        var auxL2 := Cons(x, auxL1);
+                        assert x < y;
+                        union(auxL2, ys)
+                    else
+                        if x == y then
+                            union(l1, ys)
+                        else
+                            assert x > y;
+                            lessHeadNotElems(y,l1);
+                            assert y !in elems(l1);
+                            union(Cons(y,l1),ys)
+}
+
+lemma lessHeadNotElems(y:int, l:List<int>)
+requires sorted(l)
+requires l != Nil
+ensures y < l.head ==> y !in elems(l)
+{}
+
+/////////////////////////////////
+
+function method inters (l1:List<int>,l2:List<int>): (res: List<int>)
+requires sorted(l1) && sorted(l2) && noDup(l1) && noDup(l2)
+ensures sorted(res) && noDup(res)
+ensures elems(res) == elems(l1) * elems (l2)
+{
+    match l1
+        case Nil        => Nil
+        case Cons(x,xs) =>
+            match l2
+                case Nil        => Nil
+                case Cons(y,ys) =>
+                    if x < y then
+                        lessHeadNotElems(x,l2);
+                        assert x !in elems(l2);
+                        assert sorted(inters(xs,l2));
+                        inters(xs,l2)
+                    else
+                        if x == y then
+                            sortedOrder(l1);
+                            Cons(x,inters(xs,ys))
+                        else
+                            assert y < x;
+                            lessHeadNotElems(y,l1);
+                            assert y !in elems(l1);
+                            assert sorted(inters(l1,ys));
+                            inters(l1,ys)
+}
+
+lemma sortedOrder(l:List<int>)
+requires l != Nil
+requires sorted(l) && noDup(l)
+ensures forall e | e in elems(l.tail) :: l.head < e
+{}
