liquid-haskell/session20/app/.liquid/Main.hs.bak
@@ -9,8 +9,9 @@ main :: IO()
 main = do
     putStrLn "Exercise 9.3"
     -- Get element removed
-    -- (putStrLn . show) ("isJust okRemove: " ++ show (isJust LHExercises.okRemove))
-    -- if isJust LHExercises.okRemove
-    --     then (putStrLn . show) ("fromJust okRemove: " ++ show (fst (fromJust LHExercises.okRemove)))
-    -- else (putStrLn . show) ("isNothing okRemove: " ++ show (isNothing LHExercises.okRemove))
-    -- (putStrLn . show) ("isNothing badRemove: " ++ show (isNothing LHExercises.badRemove))
+    -- (putStrLn . show) ("isJust okRemove: " ++ show (isJust LHExercises.okRemoveMaybe))
+    -- if isJust LHExercises.okRemoveMaybe
+    --     then (putStrLn . show) ("fromJust okRemove: " ++ show (fst (fromJust LHExercises.okRemoveMaybe)))
+    -- else (putStrLn . show) ("isNothing okRemove: " ++ show (isNothing LHExercises.okRemoveMaybe))
+    -- (putStrLn . show) ("isNothing badRemove: " ++ show (isNothing LHExercises.badRemoveMaybe))
+    putStrLn "Exercise 9.4"
